move GTermSem.cur to GTerm.cur (#27)

theories/lib/SAT.v
@@ -63,6 +63,15 @@ Module GTerm. Section GTerm.
     | 0 => p
     | S k' => lift (liftn k' p)
     end.
+
+  Definition cur
+    `{A : SAT.t} `{!GAT.inG A α} {n}
+    (op: A.(SAT.ops)) (args: A.(SAT.arity) op (GTerm.t_prev n) -> GTerm.t n) : GTerm.t n.
+  Proof.
+    destruct H. subst A.
+    exact (GTerm._cur inG_id op args).
+  Defined.
+
 End GTerm. End GTerm.
 
 (* Semantic Domain *)
@@ -111,6 +120,12 @@ Module GATIntp.
       inG_prf: existT _ A B = existT _ (α inG_id) (β inG_id);
     }.
   
+  #[global] Instance GATInG_GATIntpInG A α B β `{H : !inG A α B β} : GAT.inG A α :=
+    {|
+      GAT.inG_id := inG_id;
+      GAT.inG_prf := f_equal (projT1 (P := @SATIntp.t Δ α)) H.(inG_prf)
+    |}.
+
   End GSEM.
 
 End GATIntp.
@@ -139,13 +154,6 @@ Module GTermSem.
   
   Definition t n : GTerm.t n -> SemDom.dom := t_prev (S n).
 
-  Program Definition cur
-    `{A: SAT.t} `{B: @SATIntp.t Δ α A} `{IN: @GATIntp.inG Δ A α B β} {n}
-    (op: A.(SAT.ops)) (args: A.(SAT.arity) op (GTerm.t_prev n) -> GTerm.t n) : GTerm.t n.
-    destruct IN. inversion inG_prf. subst.
-    exact (GTerm._cur inG_id op args).
-  Defined.
-  
   End SEM.
   
 End GTermSem.
@@ -159,9 +167,9 @@ Module SATRed.
   Context `{β: @GATIntp.t Δ α}.
 
   Lemma cur `{A: SAT.t} `{B: @SATIntp.t Δ α A} `{IN: @GATIntp.inG Δ A α B β} n op args:
-    GTermSem.t n (GTermSem.cur op args) = B n op args (compose (GTermSem.t n) args).
+    GTermSem.t n (GTerm.cur op args) = B n op args (compose (GTermSem.t n) args).
   Proof using.
-    destruct IN eqn : EQ. subst. dependent destruction inG_prf. reflexivity.
+    destruct IN. dependent destruction inG_prf. reflexivity.
   Qed.
 
   Lemma lift_0 t d:
@@ -176,7 +184,7 @@ Module SATRed.
 
 End SATRed.
 
-Global Opaque GTermSem.cur.
+Global Opaque GTerm.cur.
 Global Opaque GTermSem.t.
 
 (** Notations *)
@@ -189,7 +197,7 @@ Local Open Scope SAT_scope.
 
 Notation "'⟦' F ',' n '⟧'" := (GTermSem.t n F).
 Notation "'⟦' F '⟧'" := (GTermSem.t _ F).
-Notation "'⟨' op ',' args '⟩'" := (GTermSem.cur op args) : SAT_scope.
+Notation "'⟨' op ',' args '⟩'" := (GTerm.cur op args) : SAT_scope.
 Notation "⤉ P" := (GTerm.lift P) (at level 20) : SAT_scope.
 
 (* Simple reduction tactics. *)
